OOM-specialized InterpProp (#335)
* remove returns WF condition: OOM spec does not satisfy it, can work around with other correctness assumptions

* small progress

* generalize k_spec and interp_prop with parameterized relation

* make interp prop more concrete, wip

* bind_Refine

* more progress, using bisim_is_eq for now

* bind closure

* more repair

* refl instanceg

* generalize R on interp_prop eutt, need another closure property

* wip new compatibility

* another checkpoint

* new compat lemma proved.. let's see if this helps with transitivity

* progress?

* check

* transitivity for oom proved; wip interp prop repair with definition change

* more repair

* more rep all OOM-related lemmas QED

* generalize types a bit

* nits

* oops, delete coqmakefiles

* update gitignore with coqmakefiles shenans

* update

* QED obligations in TopLevelRefinements except concretize_uvalue_err_oom_to_itree

* reprove convert tree for refine_h

* reprove bind clo for refine_h, apply transitivity to top level lemmas

* nits

* update gitignore

src/coq/Handlers/OOM.v
@@ -3,7 +3,8 @@ From Coq Require Import
      Relations
      String
      RelationClasses
-     Morphisms.
+     Morphisms
+     Program.Equality.
 
 From ExtLib Require Import
      Structures.Monads.
@@ -17,6 +18,9 @@ From Vellvm Require Import
 From ITree Require Import
      ITree
      Eq.Eq.
+
+From ITree Require Import Eq.EqAxiom.
+From Paco Require Import paco.
 
 Set Implicit Arguments.
 Set Contextual Implicit.
@@ -37,12 +41,6 @@ Section PARAMS_MODEL.
   Notation Effin := (E +' OOME +' F).
   Notation Effout := (E +' OOME +' F).
 
-  Definition E_trigger_model_prop : E ~> PropT Effout :=
-    fun R e => fun t => t = trigger e.
-
-  Definition F_trigger_model_prop : F ~> PropT Effout :=
-    fun R e => fun t => t = trigger e.
-
   (* Semantics of OOM *)
 
   (*    If the target tree has an out of memory event, then it is a *)
@@ -52,9 +50,6 @@ Section PARAMS_MODEL.
   (*    agree with the source at all points, but may abort, running out *)
   (*    of memory at any point. *)
   (*  *)
-  Definition OOM_handler : OOME ~> PropT Effout
-    (* Any tree is accepted as long as OOM is raised *)
-    := fun T oome source => True.
 
   Definition oom_k_spec
              {T R : Type}
@@ -68,7 +63,6 @@ Section PARAMS_MODEL.
     | _ => t2 ≈ (bind ta k2)
     end.
 
-  From Paco Require Import paco.
   #[global] Instance oom_k_spec_proper {T R : Type} {RR : R -> R -> Prop} :
     Proper
       (eq ==>
@@ -84,30 +78,200 @@ Section PARAMS_MODEL.
     all : eapply eutt_clo_bind; [ reflexivity | intros; subst; eauto ; symmetry; eauto ].
   Qed .
 
-  Definition oom_k_spec_correct_trigger:
-    k_spec_correct (fun (T : Type) (e : Effout T) => trigger e) (@oom_k_spec).
-  Proof.
-    unfold k_spec_correct.
-    intros T R [e | [e | e]] k1 k2 t2 H; cbn; auto.
-  Qed.
-
   Definition refine_OOM_handler : Effin ~> PropT Effout
-    := case_ E_trigger_model_prop (case_ OOM_handler F_trigger_model_prop).
+    := fun _ e x => x ≈ trigger e.
+
+  Definition refine_OOM_h_flip {T} (RR : relation T) (source target : itree Effout T) : Prop
+    := @interp_prop Effin Effout OOME _ refine_OOM_handler _ _ RR source target.
+
+  Arguments refine_OOM_h_flip /.
 
   Definition refine_OOM_h {T} (RR : relation T) (source target : itree Effout T) : Prop
-    := interp_prop (Basics.flip RR) refine_OOM_handler (@oom_k_spec) target source.
+    := refine_OOM_h_flip (flip RR) target source.
 
   Definition refine_OOM {T} (RR : relation T) (sources : PropT Effout T) (target : itree Effout T) : Prop
     := exists source, sources source /\ refine_OOM_h RR source target.
+
+  Ltac abs :=
+    match goal with
+    | [ H : ?t ≅ _ , H' : observe ?t = _ |- _] =>
+        rewrite (itree_eta t) in H; rewrite H' in H;
+        try solve [eapply eqit_inv in H; contradiction]
+    end.
+
+  #[global] Instance refine_OOM_h_flip_transitive {R} {RR : relation R} `{Transitive _ RR} : Transitive (refine_OOM_h_flip RR).
+  Proof.
+    unfold Transitive.
+
+    unfold refine_OOM_h_flip.
+    pcofix CIH. intros x y z EQl EQr.
+    punfold EQl; punfold EQr; red in EQl, EQr.
+    pose proof (itree_eta x) as HX; apply bisimulation_is_eq in HX; rewrite HX; clear HX.
+    pose proof (itree_eta z) as HZ; apply bisimulation_is_eq in HZ; rewrite HZ; clear HZ.
+
+    hinduction EQl before x; intros.
+    - remember (RetF r2).
+      hinduction EQr before x; intros; inv Heqi; pstep; try constructor; eauto; try abs.
+      specialize (IHEQr y _ _ REL eq_refl). punfold IHEQr.
+    - (* tau tau *)
+      assert (DEC: (exists m3, observe z= TauF m3) \/ (forall m3, observe z <> TauF m3)).
+      { destruct (observe z); eauto; right; red; intros; inv H0. }
+      destruct DEC as [EQ | EQ].
+      + destruct EQ as [m3 ?]; subst.
+        pstep. rewrite H0. econstructor; eauto. right. pclearbot.
+        rewrite H0 in EQr.
+        eapply CIH; eauto.
+        eapply interp_prop_inv_tau; eauto; pstep; auto.
+      + pclearbot.
+        inv EQr; try (exfalso; eapply EQ; eauto; fail).
+        * clear CHECK.
+          pstep; constructor; auto.
+          punfold HS. red in HS. cbn.
+          hinduction HS0 before CIH; intros; try (exfalso; eapply EQ; eauto; fail); try inv Heqot.
+          -- remember (RetF r1) as ot.
+             hinduction HS before CIH; intros; try (exfalso; eapply EQ; eauto; fail); inv Heqot.
+             ++ constructor. etransitivity; eauto.
+             ++ constructor; eauto.
+             ++ apply bisimulation_is_eq in HT1. rewrite HT1.
+                econstructor. reflexivity.
+             ++ red in H0. rewrite itree_eta in H1.
+                rewrite H3 in H1. rewrite H0 in H1.
+                setoid_rewrite bind_trigger in H1.
+                eapply eqit_inv in H1; inv H1.
+          -- eapply IHHS0; eauto.
+             assert (refine_OOM_h_flip RR t3 (Tau t1)) by (pstep; apply HS).
+             eapply interp_prop_inv_tau_r in H0; punfold H0.
+          -- apply bisimulation_is_eq in HT1. rewrite HT1 in HS.
+             cbn in HS. remember (VisF (subevent A e) k1).
+             hinduction HS before CIH; intros; try (exfalso; eapply EQ; eauto; fail); inv Heqi.
+             ++ constructor; eauto.
+             ++ apply bisimulation_is_eq in HT1. rewrite HT1; econstructor; reflexivity.
+             ++ rewrite itree_eta in H1; rewrite H3 in H1.
+                red in H0; rewrite H0 in H1. setoid_rewrite bind_trigger in H1.
+                apply eqit_inv in H1; cbn in H1.
+                destruct H1 as (?&?&?); subst. cbn in H1.
+                unfold subevent in H1.
+                unfold subevent, resum, ReSum_id, id_, ReSum_inr, cat, Id_IFun, Cat_IFun, inr_,
+                  resum , ReSum_inl , cat, resum, Inr_sum1, inl_, Inl_sum1 in H1. inv H1.
+                change (VisF (inr1 (inl1 e0)) k1) with (observe (Vis (inr1 (inl1 e0)) k1)).
+                eapply Interp_PropT_Vis_OOM. unfold subevent.
+                apply eqit_Vis. reflexivity.
+          -- red in H0. rewrite H0 in H1.
+             remember (VisF e k1). rewrite itree_eta in H1.
+             hinduction HS before CIH; intros; try (exfalso; eapply EQ; eauto; fail); try solve [inv Heqi].
+             ++ constructor; eauto.
+             ++ apply bisimulation_is_eq in HT1. rewrite HT1; econstructor; reflexivity.
+             ++ rewrite itree_eta in H1. rewrite Heqi in H1.
+                red in H0. rewrite H0 in H1. setoid_rewrite bind_trigger in H1.
+                apply eqit_inv in H1. cbn in H1. rewrite <- itree_eta in H3.
+                destruct H1 as (?&?&?); subst. cbn in H1.
+                unfold subevent in H1.
+                unfold subevent, resum, ReSum_id, id_, ReSum_inr, cat, Id_IFun, Cat_IFun, inr_,
+                  resum , ReSum_inl , cat, resum, Inr_sum1, inl_, Inl_sum1 in H1. inv H1.
+                eapply Interp_PropT_Vis. 3 : eauto. 2 : red; reflexivity. red in H3.
+
+                setoid_rewrite H0 in HK. setoid_rewrite H2 in HK0.
+                intros; right; eapply CIH; pclearbot; eauto.
+                specialize (HK _ H1); pclearbot; eauto.
+                specialize (HK0 _ H1); pclearbot; eauto.
+                specialize (H4 a). rewrite <- H4. auto.
+        * exfalso. rewrite itree_eta in HT1. rewrite H1 in HT1.
+          apply eqit_inv in HT1; inv HT1.
+    - (* tauL *)
+      specialize (IHEQl _ EQr).
+      pstep; constructor; punfold IHEQl.
+    - (* tauR *)
+      assert (refine_OOM_h_flip RR (Tau t2) z). { pstep; auto. }
+      red in H0. apply interp_prop_inv_tau_l in H0.
+      punfold H0.
+    - (* oom *)
+      apply bisimulation_is_eq in HT1. rewrite HT1; pstep; econstructor.
+      rewrite <- itree_eta; reflexivity.
+    - rewrite itree_eta in H1.
+      hinduction EQr before z; intros; try inv Heqi; pclearbot.
+      + red in H0. rewrite H0 in H1. apply eqit_inv in H1; inv H1.
+      + pstep; constructor; eauto.
+        red in H0. rewrite H0 in H1.
+        rewrite tau_eutt in H1. setoid_rewrite bind_vis in H1.
+        setoid_rewrite bind_ret_l in H1.
+        assert (refine_OOM_h_flip RR t1 t0). do 2 red. apply HS.
+        unfold refine_OOM_h_flip in H2. rewrite H1 in H2.
+        clear HS.
+        punfold H2; red in H2; cbn in H2.
+        remember (VisF (subevent A e) (fun x : A => k2 x)).
+        hinduction H2 before z; intros; try inv Heqi; pclearbot.
+        * constructor; auto; eapply IHinterp_PropTF.
+        * rewrite itree_eta in HT1. rewrite H3 in HT1.
+          apply eqit_inv in HT1. cbn in HT1. destruct HT1 as (?&?&?).
+          subst. cbn in H2.
+          eapply Interp_PropT_Vis_OOM.
+          unfold subevent, resum, ReSum_id, id_, ReSum_inr, cat, Id_IFun, Cat_IFun, inr_,
+            resum , ReSum_inl , cat, resum, Inr_sum1 in H2. inv H2.
+          apply eqit_Vis. intros; reflexivity.
+        * dependent destruction H6.
+          eapply Interp_PropT_Vis; eauto.
+          red in H2. rewrite H2 in H3. setoid_rewrite bind_trigger in H3.
+          intros. right; eapply CIH; eauto.
+          unfold subevent in H2.
+          unfold subevent, resum, ReSum_id, id_, ReSum_inr, cat, Id_IFun, Cat_IFun, inr_,
+            resum , ReSum_inl , cat, resum, Inr_sum1 in H2.
+          rewrite H2, <- H0 in H4.
+          specialize (HK _ H4); pclearbot. apply HK.
+          specialize (HK0 _ H4); pclearbot. apply HK0.
+      + eapply IHEQr. rewrite <- itree_eta. rewrite tau_eutt in H1; auto.
+      + specialize (IHEQr H1).
+        pstep; constructor; auto. punfold IHEQr.
+      + rewrite <- itree_eta in H1. rewrite HT1 in H1. red in H0.
+        rewrite H0 in H1. setoid_rewrite bind_trigger in H1.
+        apply eqit_inv in H1. cbn in H1.
+        destruct H1 as (?&?&?); subst.
+        pstep.
+        eapply Interp_PropT_Vis_OOM. red in H1.
+        unfold subevent, resum, ReSum_id, id_, ReSum_inr, cat, Id_IFun, Cat_IFun, inr_,
+          resum , ReSum_inl , cat, resum, Inr_sum1 in H1. inv H1.
+        apply eqit_Vis. intros; reflexivity.
+      + pstep.
+        red in H0; rewrite H0 in H1; setoid_rewrite bind_trigger in H1.
+        apply eqit_inv in H1; cbn in H1.
+        destruct H1 as (?&?&?); subst. cbn in H1.
+        unfold subevent in H1.
+        unfold subevent, resum, ReSum_id, id_, ReSum_inr, cat, Id_IFun, Cat_IFun, inr_,
+          resum , ReSum_inl , cat, resum, Inr_sum1, inl_, Inl_sum1 in H1. inv H1.
+        cbn in *. red in H2.
+        eapply Interp_PropT_Vis; eauto.
+        2 : rewrite <- itree_eta; eauto.
+        intros. right. eapply CIH; eauto.
+        rewrite H2 in H1; setoid_rewrite H0 in HK; specialize (HK _ H1); pclearbot; eauto.
+        specialize (HK0 _ H1); pclearbot; rewrite <- H4; eauto.
+  Qed.
 
   #[global] Instance refine_OOM_h_reflexive {R} {RR : relation R} `{Reflexive _ RR} : Reflexive (refine_OOM_h RR).
   Proof.
     unfold Reflexive.
 
-    unfold refine_OOM_h. intros x.
-    apply interp_prop_refl; try typeclasses eauto.
-    - intros X [e | [oom | f]]; reflexivity.
-    - apply oom_k_spec_correct_trigger.
+    pcofix CIH. intros t.
+    assert (t ≅ t) by reflexivity.
+    punfold H0; red in H0; intros.
+    pstep; red.
+    hinduction H0 before t; try solve [constructor; auto]; try inv CHECK; intros.
+    cbn.
+    destruct e as [e | [ oom | f]].
+    - change (VisF (inl1 e) k2) with (observe (Vis (inl1 e) k2)).
+      eapply Interp_PropT_Vis; eauto. red; reflexivity.
+      setoid_rewrite bind_trigger; reflexivity.
+    - change (VisF (inr1 (inl1 oom)) k2) with (observe (Vis (inr1 (inl1 oom)) k2)).
+      eapply Interp_PropT_Vis_OOM. eapply eqit_Vis. intros; reflexivity.
+    - change (VisF (inr1 (inr1 f)) k2) with (observe (Vis (inr1 (inr1 f)) k2)).
+      eapply Interp_PropT_Vis; eauto. red; reflexivity.
+      setoid_rewrite bind_trigger; reflexivity.
+  Qed.
+
+  #[global] Instance refine_OOM_h_transitive {R} {RR : relation R} `{Transitive _ RR} : Transitive (refine_OOM_h RR).
+  Proof.
+    unfold refine_OOM_h.
+    assert (Transitive (flip RR)).
+    { repeat intro. subst. unfold flip in *; etransitivity; eauto. }
+    repeat intro. etransitivity; eauto.
   Qed.
 
 End PARAMS_MODEL.
@@ -136,9 +300,6 @@ Section PARAMS_INTERP.
 
 End PARAMS_INTERP.
 
-Instance OOM_k_spec_WF E F : k_spec_WF (refine_OOM_handler (F:=F)) (@oom_k_spec E F).
-Admitted.
-
 Lemma eutt_refine_oom_h :
   forall {T} {E F} (RR : relation T) `{REF: Reflexive _ RR} `{TRANS : Transitive _ RR}
     (t1 t2 : itree (E +' OOME +' F) T),
@@ -146,18 +307,12 @@ Lemma eutt_refine_oom_h :
     refine_OOM_h RR t1 t2.
 Proof.
   intros T E F RR REF TRANS t1 t2 H.
-  (* apply eutt_flip in H. *)
   unfold refine_OOM_h.
-
   pose proof @interp_prop_Proper_eq.
   unfold Proper, respectful in H0.
 
-  eapply H0; eauto.
-  { apply eutt_flip. eauto. }
-
-  apply interp_prop_refl; eauto.
-  - intros X [e | [e | e]]; cbn; reflexivity.
-  - apply oom_k_spec_correct_trigger.
+  eapply H0; eauto. apply eutt_flip; eauto.
+  apply refine_OOM_h_reflexive; auto.
 Qed.
 
 Lemma refine_oom_h_raise_oom :
@@ -172,25 +327,17 @@ Proof.
   unfold refine_OOM_h.
 
   unfold raiseOOM.
-  eapply interp_prop_eutt_Proper. 1: typeclasses eauto.
-  rewrite bind_trigger. reflexivity. reflexivity.
+  eapply interp_prop_eutt_Proper.
+  rewrite bind_trigger. reflexivity.
+  reflexivity.
 
   red.
   pstep.
   econstructor.
 
   (* Instantiate ta *)
-  unshelve (instantiate (1:=_)).
-  exact (source;; trigger (ThrowOOM "")).
-  - cbn.
-    unfold OOM_handler.
-    auto.
-  - cbn.
-    intros a H.
-    destruct a.
-    Unshelve.
-    intros [].
-  - cbn; auto.
+  apply eqit_Vis; intros. inv u.
+  Unshelve. intro. inv H.
 Qed.
 
 #[global] Instance refine_OOM_h_eutt_Proper {T : Type} {RR : relation T} {E F}:
@@ -199,120 +346,12 @@ Proof.
   unfold Proper, respectful.
   intros x y XY z w ZW.
   split; intros REF; subst.
-  - unfold refine_OOM_h in *.
+  - unfold refine_OOM_h, refine_OOM_h_flip in *.
     rewrite ZW in REF.
     rewrite XY in REF.
     auto.
-  - unfold refine_OOM_h in *.
+  - unfold refine_OOM_h, refine_OOM_h_flip in *.
     rewrite <- ZW in REF.
     rewrite <- XY in REF.
     auto.
 Qed.
-
-
-(* Instance Transitive_refine_OOM_h {E F T} {RR} : Transitive (@refine_OOM_h E F T RR). *)
-(* Proof. *)
-(*   unfold Transitive. *)
-(*   intros x y z XY YZ. *)
-
-(*   epose proof interp_prop_Proper3. *)
-(*   epose proof interp_prop_Proper2. *)
-(*   epose proof interp_prop_Proper. *)
-(*   unfold Proper, respectful in *. *)
-
-
-(*   pose proof (itree_eta x) as Ix. *)
-(*   pose proof (itree_eta y) as Iy. *)
-(*   pose proof (itree_eta z) as Iz. *)
-
-(*   unfold refine_OOM_h in *. *)
-(*   eapply H. *)
-(*   3: eapply XY. *)
-(*   all:eauto. *)
-
-
-(*   destruct (observe z) eqn:Hz. *)
-(*   - pstep. red. *)
-
-(*     destruct (observe y) eqn:Hy. *)
-(*     + unfold refine_OOM_h in *. *)
-
-(*       assert (y = ret r1) by admit. *)
-(*       rewrite H in YZ. *)
-(*       rewrite H in XY. *)
-(*       clear H. *)
-
-(*       assert (z = ret r0) by admit. *)
-(*       rewrite H in YZ. *)
-(*       clear H. *)
-
-(*       apply interp_prop_ret_inv in XY as (rx & RRx & REST). *)
-(*       unfold flip in RRx. *)
-
-(*       apply  *)
-(*       replace y with (ret r1) in YZ. *)
-(*       rewrite Ix in XY. *)
-
-
-(*        to *)
-
-(*       unfold interp_prop in *. *)
-(*   epose proof interp_prop_Proper. *)
-(*   unfold Proper, respectful in H. *)
-(*   generalize dependent x. *)
-(*   generalize depy, z. *)
-(*   pcofix  *)
-(*   unfold Basics.flip, Basics.impl in H. *)
-(*   eapply H. *)
-(*   admit. *)
-(*   admit. *)
-(* Qed. *)
-
-(* Instance Transitive_refine_OOM_h {E F T} {RR} : Transitive (@refine_OOM_h E F T RR). *)
-(* Proof. *)
-(*   unfold Transitive. *)
-(*   Require Import Paco.paco. *)
-
-(*   pcofix CIH. *)
-(*   intros x y z XY YZ. *)
-
-(*   pose proof (itree_eta x) as Ix. *)
-(*   pose proof (itree_eta y) as Iy. *)
-(*   pose proof (itree_eta z) as Iz. *)
-
-(*   destruct (observe z) eqn:Hz. *)
-(*   - pstep. red. *)
-
-(*     destruct (observe y) eqn:Hy. *)
-(*     + unfold refine_OOM_h in *. *)
-
-(*       assert (y = ret r1) by admit. *)
-(*       rewrite H in YZ. *)
-(*       rewrite H in XY. *)
-(*       clear H. *)
-
-(*       assert (z = ret r0) by admit. *)
-(*       rewrite H in YZ. *)
-(*       clear H. *)
-
-(*       apply interp_prop_ret_inv in XY as (rx & RRx & REST). *)
-(*       unfold flip in RRx. *)
-
-(*       apply  *)
-(*       replace y with (ret r1) in YZ. *)
-(*       rewrite Ix in XY. *)
-
-
-(*        to *)
-
-(*       unfold interp_prop in *. *)
-(*   epose proof interp_prop_Proper. *)
-(*   unfold Proper, respectful in H. *)
-(*   generalize dependent x. *)
-(*   generalize depy, z. *)
-(*   pcofix  *)
-(*   unfold Basics.flip, Basics.impl in H. *)
-(*   eapply H. *)
-(*   admit. *)
-(*   admit. *)
-(* Qed. *)
