src/coq/Utils/InterpProp.v
@@ -24,7 +24,8 @@ From Coq Require Import
      List
      Program.Tactics Program.Equality.
 From ITree Require Import
-     Basics.Monad.
+     Basics.Monad
+     Eq.EqAxiom.
 
 From Vellvm Require Import
      Utils.PropT.
@@ -39,108 +40,65 @@ Local Open Scope monad_scope.
 Local Open Scope cat_scope.
 (* end hide *)
 
+(* Definition 5.3: Handler Correctness *)
+  Definition handler_correct {E F} (h_spec: E ~> PropT F) (h: E ~> itree F) :=
+    (forall T e ta, ta ≈ h T e -> h_spec T e ta).
+
+#[global] Instance void1_unit {E} : void1 -< E.
+  repeat intro; contradiction.
+Qed.
+
 Section interp_prop.
 
-  (* Definition 5.3: Handler Correctness *)
-  Definition handler_correct {E F} (h_spec: E ~> PropT F) (h: E ~> itree F) :=
-    (forall T e ta, ta ≈ h T e <-> h_spec T e ta).
-
-  Lemma case_prop_handler_correct:
-    forall {E1 E2 F}
-      (h1_spec: E1 ~> PropT F)
-      (h2_spec: E2 ~> PropT F)
-      (h1: E1 ~> itree F)
-      (h2: E2 ~> itree F)
-      (C1: handler_correct h1_spec h1)
-      (C2: handler_correct h2_spec h2),
-      handler_correct (case_ h1_spec h2_spec) (case_ h1 h2).
-  Proof.
-    intros E1 E2 F h1_spec h2_spec h1 h2 C1 C2.
-    unfold handler_correct in *.
-    intros T e.
-    destruct e. apply C1. apply C2.
-  Qed.
-
-  Definition k_spec_correct
-             {E F}
-             (h: E ~> itree F)
-             (k_spec : forall T R, E T -> itree F T -> (T -> itree F R) -> itree F R -> Prop) : Prop
-    := forall T R e k2 t2 ta, ta ≈ h _ e -> t2 ≈ bind ta k2 -> k_spec T R e ta k2 t2.
-
-  Context {E F : Type -> Type}.
-  Context {R1 R2 : Type} (RR : R1 -> R2 -> Prop).
-  Context (h_spec : E ~> PropT F).
-  Context (k_spec : forall T R, E T -> itree F T -> (T -> itree F R) -> itree F R -> Prop).
-
-  (* Well-formedness conditions for k_specs *)
-  Class k_spec_WF := {
-      k_spec_Returns: forall {A R} ta k2 t2 e,
-        k_spec A R e ta k2 t2 -> forall a, Returns a ta -> forall a', Returns a' (k2 a) -> Returns a' t2;
-      k_spec_bind: forall {A R1 R2} ta k2 (t2 : itree F _) e (k' : R1 -> itree F R2),
-        k_spec A _ e ta k2 t2 ->
-        k_spec A _ e ta (fun x => bind (k2 x) k') (bind t2 k');
-      k_spec_Proper : forall {A R} ta k e,
-        Proper (eutt eq ==> iff) (k_spec A R e ta k);
-      k_spec_respects_h_spec : forall {A} (ta : itree F _) (k : _ -> itree F _) e x,
-           ta ≈ x <- ta ;; k x ->
-           k_spec A _ e ta k x ->
-           h_spec _ e ta ->
-           h_spec _ e x
-    }.
-
-  Context `{k_spec_wellformed : k_spec_WF}.
+  Context {E F OOM : Type -> Type} {OOME: OOM -< E}.
+  Context (h_spec : E ~> PropT F) {R1 R2 : Type} (RR : R1 -> R2 -> Prop).
 
   Inductive interp_PropTF
-            (b1 b2 : bool)
-            (vclo : (itree E R1 -> itree F R2 -> Prop) -> itree E R1 -> itree F R2 -> Prop)
-            (sim : itree E R1 -> itree F R2 -> Prop)
+            (b1 b2 : bool) (sim : itree E R1 -> itree F R2 -> Prop)
             : itree' E R1 -> itree' F R2 -> Prop :=
   | Interp_PropT_Ret : forall r1 r2 (REL: RR r1 r2),
-      interp_PropTF b1 b2 vclo sim (RetF r1) (RetF r2)
+      interp_PropTF b1 b2 sim (RetF r1) (RetF r2)
 
   | Interp_PropT_Tau : forall t1 t2 (HS: sim t1 t2),
-      interp_PropTF b1 b2 vclo sim (TauF t1) (TauF t2)
+      interp_PropTF b1 b2 sim (TauF t1) (TauF t2)
 
   | Interp_PropT_TauL : forall t1 t2
                           (CHECK: is_true b1)
-                          (HS: interp_PropTF b1 b2 vclo sim (observe t1) t2),
-      interp_PropTF b1 b2 vclo sim (TauF t1) t2
+                          (HS: interp_PropTF b1 b2 sim (observe t1) t2),
+      interp_PropTF b1 b2 sim (TauF t1) t2
 
   | Interp_PropT_TauR : forall t1 t2
                           (CHECK: is_true b2)
-                          (HS: interp_PropTF b1 b2 vclo sim t1 (observe t2)),
-      interp_PropTF b1 b2 vclo sim t1 (TauF t2)
+                          (HS: interp_PropTF b1 b2 sim t1 (observe t2)),
+      interp_PropTF b1 b2 sim t1 (TauF t2)
 
-  | Interp_PropT_Vis : forall A (e : E A) (k1 : A -> itree E R1) ta
-                         (t2 : itree F R2)
+  | Interp_PropT_Vis_OOM : forall A (e : OOM A) k1 t1 t2
+                         (HT1: t1 ≅ vis e k1),
+      interp_PropTF b1 b2 sim (observe t1) t2
 
-                         (k2 : A -> itree F R2)
-
-                         (HTA: h_spec A e ta)
-                         (HK : forall (a : A), Returns a ta -> vclo sim (k1 a) (k2 a))
-
-                         (KS : k_spec A R2 e ta k2 t2),
-      interp_PropTF b1 b2 vclo sim (VisF e k1) (observe t2).
+  | Interp_PropT_Vis : forall A e k1 k2 (ta t2 : itree F _)
+                  (HK : forall (a : A), Returns a ta -> sim (k1 a) (k2 a)),
+        h_spec _ e ta ->
+        t2 ≈ ta >>= k2 ->
+        interp_PropTF b1 b2 sim (VisF e k1) (observe t2).
 
   Hint Constructors interp_PropTF : core.
 
-  Lemma interp_PropTF_mono b1 b2 x0 x1 vclo vclo' sim sim'
-        (IN: interp_PropTF b1 b2 vclo sim x0 x1)
-        (MON: monotone2 vclo)
-        (LEc: vclo <3= vclo')
+  Lemma interp_PropTF_mono b1 b2 x0 x1 sim sim'
+        (IN: interp_PropTF b1 b2 sim x0 x1)
         (LE: sim <2= sim'):
-    interp_PropTF b1 b2 vclo' sim' x0 x1.
+    interp_PropTF b1 b2 sim' x0 x1.
   Proof.
     intros. induction IN; eauto.
   Qed.
 
   Hint Resolve interp_PropTF_mono : paco.
 
-  Definition interp_PropT_ b1 b2 vclo sim (t0 : itree E R1) (t1 : itree F R2) :=
-    interp_PropTF b1 b2 vclo sim (observe t0) (observe t1).
+  Definition interp_PropT_ b1 b2 sim (t0 : itree _ R1) (t1 : itree _ R2) :=
+    interp_PropTF b1 b2 sim (observe t0) (observe t1).
   Hint Unfold interp_PropT_ : core.
 
-  Lemma interp_PropT__mono b1 b2 vclo (MON: monotone2 vclo) : monotone2 (interp_PropT_ b1 b2 vclo).
+  Lemma interp_PropT__mono b1 b2 : monotone2 (interp_PropT_ b1 b2).
   Proof.
     do 2 red. intros. eapply interp_PropTF_mono; eauto.
   Qed.
@@ -152,96 +110,24 @@ Section interp_prop.
 
   (* Definition 5.2 *)
   Definition interp_prop' b1 b2 :
-    itree E R1 -> PropT F R2 :=
-    paco2 (interp_PropT_ b1 b2 id) bot2.
+    itree _ R1 -> PropT _ R2 :=
+    paco2 (interp_PropT_ b1 b2) bot2.
 
   Definition interp_prop :
-    itree E R1 -> PropT F R2 :=
+    itree _ R1 -> PropT _ R2 :=
     interp_prop' true true.
 
   #[global] Instance interp_prop_eq_itree_Proper_impl_ :
     forall (x : _ R1), Proper (eq_itree eq ==> impl) (interp_prop x).
   Proof.
-    repeat intro. red in H0.
-    punfold H; punfold H0; red in H; red in H0; cbn in *.
-    revert_until k_spec_wellformed.
-    pcofix CIH.
-    intros x y y' EQ H.
-    remember (observe x); remember (observe y).
-    revert x Heqi y y' Heqi0 EQ.
-    (* induct on interp_prop *)
-    induction H; subst; pclearbot; intros.
-    - inv EQ; [ | inv CHECK].
-      pstep. red. rewrite <- Heqi, <- H.
-      eauto.
-    - inv EQ; try inv CHECK; pclearbot.
-      pstep. red. rewrite <- Heqi, <- H.
-      constructor. right. eapply CIH; eauto.
-      punfold REL. punfold HS.
-    - pstep. red. rewrite <- Heqi. constructor; auto.
-      specialize (IHinterp_PropTF _ eq_refl _ _ Heqi0 EQ).
-      punfold IHinterp_PropTF.
-    - pstep. red. rewrite <- Heqi.
-      inv EQ; try inv CHECK0; pclearbot.
-      constructor; auto. punfold REL.
-      specialize (IHinterp_PropTF _ eq_refl _ m2 eq_refl REL).
-      punfold IHinterp_PropTF.
-    - pstep. red. rewrite <- Heqi.
-      econstructor; eauto; cycle 1.
-      eapply k_spec_Proper. symmetry.
-      assert (t2 ≅ y') by (pstep; auto).
-      rewrite <- H. reflexivity. eauto.
-      intros. specialize (HK _ H). pclearbot.
-      left. eapply paco2_mon; intros; eauto.
-      inv PR.
+    repeat intro. eapply bisimulation_is_eq in H; subst; eauto.
   Qed.
 
   #[global] Instance interp_prop_eq_itree_Proper_impl :
     Proper (eq_itree eq ==> eq_itree eq ==> impl) interp_prop.
   Proof.
     repeat intro.
-    rewrite <- H0. clear H0.
-    clear y0. rename H1 into H0. rename y into x'. rename x0 into y.
-    punfold H; punfold H0; red in H; red in H0; cbn in *.
-    revert_until k_spec_wellformed.
-    pcofix CIH.
-    intros x x' EQ y H.
-    remember (observe x); remember (observe y).
-    revert x x' Heqi y Heqi0 EQ.
-    (* induct on interp_prop *)
-    induction H; subst; pclearbot; intros.
-    - inv EQ; [ | inv CHECK].
-      pstep. red. rewrite <- Heqi0, <- H.
-      eauto.
-    - inv EQ; try inv CHECK; pclearbot.
-      pstep. red. rewrite <- Heqi0, <- H.
-      constructor. right. eapply CIH; eauto.
-      punfold REL. punfold HS.
-    - pstep. red. rewrite <- Heqi0.
-      inv EQ; try inv CHECK0; pclearbot.
-      constructor; auto. punfold REL.
-      specialize (IHinterp_PropTF _ _ eq_refl _ eq_refl REL).
-      punfold IHinterp_PropTF.
-    - pstep. red. rewrite <- Heqi0. constructor; auto.
-      specialize (IHinterp_PropTF _ _ Heqi _ eq_refl EQ).
-      punfold IHinterp_PropTF.
-    - pstep.
-      assert (Vis e k1 ≅ x') by (pstep; auto).
-      eapply eqit_inv in H. cbn in H.
-      destruct (_observe x') eqn: Hx'; inv H.
-      red. unfold observe at 1. rewrite Hx'.
-      destruct H0. red in H. subst.
-      red in H0.
-      econstructor; eauto; cycle 1.
-      assert (t2 ≈ y).
-      { rewrite itree_eta; rewrite Heqi0; rewrite <- itree_eta; reflexivity. }
-      eapply k_spec_Proper.
-      symmetry in H; apply H.
-      exact KS.
-      intros. specialize (HK _ H). pclearbot.
-      punfold HK.
-      right. eapply CIH; eauto.
-      specialize (H0 a). punfold H0.
+    repeat intro. eapply bisimulation_is_eq in H, H0; subst; eauto.
   Qed.
 
   #[global] Instance interp_prop_eq_itree_Proper :
@@ -276,9 +162,10 @@ Section interp_prop.
       rewrite <- itree_eta in IHinterp_PropTF.
       punfold IHinterp_PropTF.
     - rewrite <- itree_eta. pstep; auto.
-    - pstep; econstructor; eauto. eapply k_spec_Proper; eauto.
-      rewrite (itree_eta t2); rewrite H0.
-      rewrite tau_eutt; reflexivity.
+    - rewrite HT1, <- itree_eta; pstep; econstructor; reflexivity.
+    - pstep; eapply Interp_PropT_Vis; eauto.
+      rewrite (itree_eta t2) in H0.
+      rewrite H2 in H0. rewrite tau_eutt in H0; eauto.
   Qed.
 
   Lemma interp_prop_inv_tau_l (t0 : _ R1) t1:
@@ -297,6 +184,7 @@ Section interp_prop.
       specialize (IHinterp_PropTF _ eq_refl _ eq_refl).
       rewrite <- itree_eta in IHinterp_PropTF.
       punfold IHinterp_PropTF.
+    - rewrite itree_eta in HT1; rewrite H0 in HT1; eapply eqit_inv in HT1; contradiction.
   Qed.
 
   Lemma interp_prop_inv_tau (t0 : _ R1) t1:
@@ -313,7 +201,7 @@ Section interp_prop.
   Proof.
     repeat intro. red in H0.
     punfold H; punfold H0; red in H; red in H0; cbn in *.
-    revert_until k_spec_wellformed.
+    revert_until RR.
     pcofix CIH.
     intros x y y' EQ H.
     remember (observe x); remember (observe y).
@@ -354,15 +242,13 @@ Section interp_prop.
           hinduction HS before CIH; intros; try discriminate; eauto.
           pose proof @Interp_PropT_Vis.
           change (VisF e0 k3) with (observe (Vis e0 k3)).
-          eapply H; eauto.
+          eapply H1; eauto.
           intros.
-          left. specialize (HK _ H0). pclearbot.
+          left. specialize (HK _ H2). pclearbot.
           eapply paco2_mon; eauto. intros; inv PR.
-          eapply k_spec_Proper. eapply eqit_Vis. symmetry. pclearbot. eapply REL.
-          eapply k_spec_Proper. Unshelve.
-          3 : exact t2.
-          rewrite (itree_eta t2), Heqot. eapply eqit_Vis; reflexivity.
-          auto.
+          rewrite itree_eta in H0; rewrite Heqot in H0.
+          rewrite <- H0; apply eqit_Vis.
+          symmetry. pclearbot. eauto.
         * eapply IHREL; eauto. pstep_reverse.
           assert (interp_prop t0 (Tau t1)) by (pstep; auto).
           apply interp_prop_inv_tau_r in H. punfold H.
@@ -377,13 +263,18 @@ Section interp_prop.
       assert (Tau t0 ≈ t2). { pstep; auto. }
       apply eqit_inv_Tau_l in H1; punfold H1.
     - rewrite <- Heqi.
-      econstructor; eauto; cycle 1.
-      eapply k_spec_Proper. rewrite Heqi0 in EQ.
-      symmetry. pstep; red; eauto.
-      eapply k_spec_Proper. 2 : eauto. rewrite itree_eta; rewrite <- Heqi0; rewrite <- itree_eta; reflexivity.
-      intros. specialize (HK _ H). pclearbot.
+      econstructor; eauto.
+    - rewrite <- Heqi.
+
+      rewrite Heqi0 in EQ.
+      rewrite itree_eta in H0.
+      rewrite Heqi0, <- itree_eta in H0; clear Heqi0.
+      econstructor; eauto.
+      intros; eauto.
+      specialize (HK _ H1). pclearbot.
       left. eapply paco2_mon; intros; eauto.
-      inv PR.
+      inv PR. assert (y ≈ y') by (pstep; auto).
+      rewrite <- H1; auto.
   Qed.
 
   #[global] Instance interp_prop_eutt_Proper_impl :
@@ -392,7 +283,7 @@ Section interp_prop.
     intros y y' EQ x x' EQ' H.
     rewrite <- EQ'. clear x' EQ'.
     punfold H; punfold EQ; red in H; red in EQ; cbn in *.
-    revert_until k_spec_wellformed.
+    revert_until RR.
     pcofix CIH.
     intros x x' EQ y H.
     remember (observe x); remember (observe y).
@@ -431,13 +322,23 @@ Section interp_prop.
           intros; left; pclearbot; eapply paco2_mon; eauto; intros; inv PR0.
         * remember (VisF e k1) as ot.
           hinduction HS before CIH; intros; try discriminate; eauto.
-          pose proof @Interp_PropT_Vis.
-          inversion Heqot. dependent destruction H3.
-          eapply H; eauto.
-          intros. right. eapply CIH; eauto.
-          specialize (REL a). pclearbot. punfold REL.
-          specialize (HK _ H0). pclearbot.
-          punfold HK.
+          -- pose proof @Interp_PropT_Vis.
+              inversion Heqot.
+              rewrite itree_eta in HT1; rewrite Heqot in HT1.
+              eapply eqit_inv in HT1. cbn in HT1. destruct HT1 as (?&?&?).
+              subst. cbn in *. inv H0.
+              match goal with
+              | |- interp_PropTF _ _ _  ?l _ => change l with (observe (go l))
+              end.
+              eapply Interp_PropT_Vis_OOM; reflexivity.
+          -- inv Heqot.
+             dependent destruction H3. econstructor.
+             2, 3: eauto.
+             intros. right.
+             eapply CIH; eauto.
+              specialize (REL a). pclearbot. punfold REL.
+              specialize (HK _ H1). pclearbot.
+              punfold HK.
         * eapply IHREL; eauto. pstep_reverse.
           assert (interp_prop (Tau t0) t2) by (pstep; auto).
           apply interp_prop_inv_tau_l in H. punfold H.
@@ -447,16 +348,23 @@ Section interp_prop.
       punfold H0.
     - rewrite <- Heqi0.
       constructor; auto. eapply IHinterp_PropTF; eauto.
-    - rewrite <- Heqi0.
-      remember (VisF e k1). clear x Heqi.
-
-      hinduction EQ before CIH; intros; try inversion Heqi1; pclearbot; subst; eauto.
-      dependent destruction H1.
-      econstructor; eauto.
-      intros; specialize (HK _ H); pclearbot.
-      right; eapply CIH; [ | punfold HK].
-      specialize (REL a).
-      punfold REL.
+    - rewrite <- Heqi0. rewrite itree_eta in HT1.
+      hinduction EQ before CIH; intros; try inversion Heqi1; pclearbot;
+        subst; eauto; apply eqit_inv in HT1; try inv HT1.
+      destruct H as (?&?). cbn in *. inv H.
+      match goal with
+      | |- interp_PropTF _ _ _  ?l _ => change l with (observe (go l))
+      end.
+      eapply Interp_PropT_Vis_OOM; reflexivity.
+    - rewrite Heqi in EQ.
+      hinduction EQ before CIH; intros; try inversion Heqi1; pclearbot; inv Heqi.
+      + dependent destruction H3.
+        econstructor; eauto.
+        intros. specialize (HK _ H1); pclearbot.
+        right; eapply CIH; [ | punfold HK].
+        specialize (REL a).
+        punfold REL. setoid_rewrite itree_eta at 1 ; rewrite <- Heqi0, <- itree_eta; auto.
+      + econstructor; eauto.
   Qed.
 
   #[global] Instance interp_prop_eutt_Proper :
@@ -464,7 +372,11 @@ Section interp_prop.
   Proof.
     split; intros; [rewrite <- H, <- H0 | rewrite H, H0]; auto.
   Qed.
+
 End interp_prop.
+
+Arguments interp_prop {_ _ _ _} _ {_ _}.
+Arguments interp_prop' {_ _ _ _} _ {_ _}.
 
 Hint Constructors interp_PropTF : core.
 Hint Resolve interp_PropTF_mono : paco.
@@ -473,128 +385,185 @@ Hint Resolve interp_PropT__mono : paco.
 Hint Resolve interp_PropT_idclo_mono : paco.
 
 #[global] Instance interp_prop_Proper_eq :
-  forall (E F : Type -> Type) (h_spec : forall T : Type, E T -> PropT F T)
-    (k_spec : forall T R : Type,
-        E T -> itree F T -> (T -> itree F R) -> itree F R -> Prop)
-    R (RR : relation R) (HR: Reflexive RR) (HT : Transitive RR),
-    Proper (@eutt _ _ _ RR ==> eq ==> flip Basics.impl) (interp_prop RR h_spec k_spec).
+  forall (E F OOM : Type -> Type) (h_spec : forall T : Type, E T -> PropT F T)
+    R (RR : R -> R -> Prop) (HR: Reflexive RR) (HT : Transitive RR) `{OOM -< E},
+    Proper (@eutt _ _ _ RR ==> eq ==> flip Basics.impl) (@interp_prop E F OOM _ h_spec _ _ RR).
 Proof.
-Admitted.
+  intros E F OOM h_spec R RR REFL TRANS CONSTRAINT.
+  intros y y' EQ x x' EQ' H. subst.
+  punfold H; punfold EQ; red in H; red in EQ; cbn in *.
+  revert_until CONSTRAINT.
+  pcofix CIH.
+  intros x x' EQ y H.
+  remember (observe x); remember (observe y).
+  pstep. red. genobs_clear x' ox'.
+  revert x Heqi y Heqi0 EQ.
+  (* induct on interp_prop *)
+  rename i into xo, i0 into yo.
+  induction H; subst; pclearbot; intros.
+  - rewrite <- Heqi0.
+    remember (RetF (E:= E) r1).
+    hinduction EQ before REL; intros; inv Heqi1; inv Heqi; intros.
+    + constructor; eauto.
+    + constructor; eauto.
 
-Lemma interp_prop_eqit_clo_wcompat {E R RR h_spec k_spec b1 b2 vclo}
-    `{k_spec_WF _ _ h_spec k_spec}
-  (MON: monotone2 vclo)
-  (CMP: compose (eqitC eq b1 b2) vclo <3= compose vclo (eqitC eq b1 b2)):
-  wcompatible2 (@interp_PropT_ E E R R RR h_spec k_spec b1 b2 vclo) (eqitC eq b1 b2).
-Proof.
-  econstructor.
-  pmonauto.
-  intros.
-  destruct PR.
-  punfold EQVl.
-  punfold EQVr.
-  unfold_eqit. red in REL.
-  hinduction REL before r; intros; clear t1' t2'; red.
-  - remember (RetF r1) as x.
-    hinduction EQVl before r; intros; subst; try inv Heqx; eauto.
-    remember (RetF r3) as y.
-    hinduction EQVr before r; intros; subst; try inv Heqy; eauto.
-    constructor. specialize (LERR1 _ _ _ REL0 eq_refl). subst.
-    specialize (LERR2 _ _ _ REL eq_refl). subst. auto.
-  - remember (TauF t1) as x.
-    hinduction EQVl before r; intros; subst; try inv Heqx; try inv CHECK; eauto.
-    remember (TauF t2) as y.
-    hinduction EQVr before r; intros; subst; try inv Heqy; try inv CHECK; eauto.
-    pclearbot. econstructor. gclo.
-    econstructor; eauto with paco.
-  - remember (TauF t1) as x.
-    hinduction EQVl before r; intros; subst; try inv Heqx; try inv CHECK; eauto.
-    pclearbot. constructor; punfold REL.
-    eapply IHREL; eauto.
-  - remember (TauF t2) as y.
-    hinduction EQVr before r; intros; subst; try inv Heqy; try inv CHECK; eauto.
-    pclearbot;constructor; punfold REL.
-    eapply IHREL; eauto.
-  - remember (VisF e k1) as x.
-    hinduction EQVl before r; intros; try discriminate Heqx; eauto; inv_Vis.
-    pclearbot.
-    econstructor; intros; cycle 1.
-    eapply MON; cycle 1.
-    + intros. apply gpaco2_clo, PR.
-    + apply CMP. econstructor. 1, 2, 3: eauto. reflexivity.
-      eauto. intros; subst; eauto.
-    + assert (t0 ≈ t2).
-      { eapply eqit_mon. 4 : pstep; eapply EQVr.
-        1, 2: eauto. intros. specialize (LERR2 _ _ _ PR eq_refl). auto. }
-      eapply k_spec_Proper; eauto.
-    + eauto.
-Qed.
+  - rewrite <- Heqi0.
+    rewrite <- Heqi. rename xo into ot3.
+    assert (DEC: (exists m3, ot3 = TauF m3) \/ (forall m3, ot3 <> TauF m3)).
+    { destruct ot3; eauto; right; red; intros; inv H. }
 
-Hint Resolve interp_prop_eqit_clo_wcompat : paco.
+    rename EQ into INR.
+    destruct DEC as [EQ | EQ].
+    + destruct EQ as [m3 H]; rewrite H.
+      econstructor. right. pclearbot. eapply CIH; eauto with paco.
+      rewrite H in INR.
+      assert (eutt RR (Tau m3) (Tau t1)) by (pstep; eauto).
+      2 : punfold HS.
+      eapply eqit_inv_Tau in H0. punfold H0.
 
-Inductive interp_prop_bind_clo {E} {R1 R2} h_spec k_spec b1 b2 (r : itree E R1 -> itree E R2 -> Prop) :
-  itree E R1 -> itree E R2 -> Prop :=
-| pbc_intro_h U1 U2 (RU : U1 -> U2 -> Prop) t1 t2 k1 k2
-      (EQV: interp_prop' RU h_spec k_spec b1 b2 t1 t2)
-      (REL: forall u1 u2, RU u1 u2 -> r (k1 u1) (k2 u2))
-  : interp_prop_bind_clo h_spec k_spec b1 b2 r (ITree.bind t1 k1) (ITree.bind t2 k2)
-.
-Hint Constructors interp_prop_bind_clo: core.
-
-Lemma interp_prop_clo_bind {E} R (RR : R -> R -> Prop) h_spec k_spec {U1 U2 UU} t1 t2 k1 k2
-      `{k_spec_WF _ _ h_spec k_spec}
-      (EQT: @interp_prop E E U1 U2 UU h_spec k_spec t1 t2)
-      (EQK: forall u1 u2, UU u1 u2 -> interp_prop RR h_spec k_spec (k1 u1) (k2 u2)):
-  interp_prop RR h_spec k_spec (ITree.bind t1 k1) (ITree.bind t2 k2).
-Proof.
-  revert_until UU.
-
-  ginit. gcofix CIH.
-  intros.
-  punfold EQT.
-  red in EQT.
-  gclo.
-  econstructor.
-  rewrite unfold_bind; reflexivity.
-  rewrite unfold_bind; reflexivity. 2,3: intros; subst; eauto.
-
-  gstep.
-  induction EQT; eauto; pclearbot.
-  - specialize (EQK _ _ REL).
-    punfold EQK.
-    eapply interp_PropTF_mono; eauto.
-    intros; eauto. pclearbot.
-    gfinal. right.
-    eapply paco2_mon; eauto.
-    intros; contradiction.
-  - constructor. gfinal. left.
-    specialize (CIH _ _ _ _ H0 HS EQK).
-    eauto.
-  - econstructor; auto.
-  - econstructor; auto.
-  - econstructor; eauto.
-    + intros. gbase; eapply CIH; eauto.
-      specialize (HK _ H). pclearbot; eauto.
-    + eapply k_spec_Proper; cycle 1.
-      * rewrite <- unfold_bind. reflexivity.
-      * pose proof @k_spec_bind as Hbind.
-        specialize (Hbind _ _ h_spec k_spec H0 _ _ _ _ _ _ _ k2 KS).
-        eapply Hbind.
-      * eauto.
+    + inv INR; try (exfalso; eapply EQ; eauto; fail).
+      econstructor; eauto.
+      punfold HS. red in HS.
+      pclearbot.
+      hinduction REL before CIH; intros; try (exfalso; eapply EQ; eauto; fail).
+      * subst. remember (RetF r2) as ot.
+        hinduction HS before r1; intros; inv Heqot.
+        -- econstructor; eauto.
+        -- econstructor; eauto.
+        -- rewrite itree_eta in HT1; rewrite H0 in HT1; apply eqit_inv in HT1; inv HT1.
+      * remember (VisF e k2) as ot.
+        hinduction HS before CIH; intros; try discriminate; eauto.
+        -- pose proof @Interp_PropT_Vis.
+            inversion Heqot.
+            rewrite itree_eta in HT1; rewrite Heqot in HT1.
+            eapply eqit_inv in HT1. cbn in HT1. destruct HT1 as (?&?&?).
+            subst. cbn in *. inv H0.
+            match goal with
+            | |- interp_PropTF _ _ _ _ _  ?l _ => change l with (observe (go l))
+            end.
+            eapply Interp_PropT_Vis_OOM; reflexivity.
+        -- inv Heqot.
+            dependent destruction H3. econstructor.
+            2, 3: eauto.
+            intros. right.
+            eapply CIH; eauto.
+            specialize (REL a). pclearbot. punfold REL.
+            specialize (HK _ H1). pclearbot.
+            punfold HK.
+      * eapply IHREL; eauto. pstep_reverse.
+        assert (interp_prop h_spec RR (Tau t2) t0) by (pstep; auto).
+        apply interp_prop_inv_tau_l in H. punfold H.
+  - specialize (IHinterp_PropTF _ Heqi _ Heqi0).
+    assert (eutt RR (go xo) t1).
+    { rewrite <- (tau_eutt t1); pstep; auto. }
+    punfold H0.
+  - rewrite <- Heqi0.
+    constructor; auto.
+  - rewrite <- Heqi0. rewrite itree_eta in HT1. rewrite <- Heqi.
+    clear x Heqi.
+    hinduction EQ before CIH; intros; try inversion Heqi1; pclearbot;
+      subst; eauto; apply eqit_inv in HT1; try inv HT1.
+    destruct H as (?&?). cbn in *. inv H.
+      match goal with
+      | |- interp_PropTF _ _ _ _ _ ?l _ => change l with (observe (go l))
+      end.
+      eapply Interp_PropT_Vis_OOM; subst. reflexivity.
+  - rewrite Heqi in EQ.
+    remember (VisF e k1).
+    hinduction EQ before CIH; intros; try inversion Heqi1; pclearbot; inv Heqi.
+    + dependent destruction H3.
+      econstructor; eauto.
+      intros. specialize (HK _ H1); pclearbot.
+      right; eapply CIH; [ | punfold HK].
+      specialize (REL a).
+      punfold REL. setoid_rewrite itree_eta at 1 ; rewrite <- Heqi0, <- itree_eta; auto.
+    + econstructor; eauto.
 Qed.
 
 Section interp_prop_extra.
 
-  Context {E F : Type -> Type}.
+  Context {E F OOM : Type -> Type} {OOME: OOM -< E}.
+  Context (h : E ~> PropT F).
   Context {R1 R2 : Type} (RR : R1 -> R2 -> Prop).
-  Context (h_spec : E ~> PropT F).
-  Context (k_spec : forall T R, E T -> itree F T -> (T -> itree F R) -> itree F R -> Prop).
-  Context `{k_spec_wellformed : @k_spec_WF _ _ h_spec k_spec}.
+
+  Lemma interp_prop_clo_bind {U} t1 t2 k1 k2
+        (EQT: @interp_prop E F OOM _ h U _ eq t1 t2)
+        (EQK: forall u1 u2, eq u1 u2 -> @interp_prop E F OOM _ h _ _ eq (k1 u1) (k2 u2)):
+    @interp_prop E F OOM _ h _ _ eq (ITree.bind t1 k1) (ITree.bind (U := U) t2 k2).
+  Proof.
+    revert_until U.
+
+    pcofix CIH.
+    intros.
+    punfold EQT.
+    red in EQT.
+
+    assert (ITree.bind t1 k1 =
+              match observe t1 with
+              | RetF r => k1 r
+              | TauF t0 => Tau (ITree.bind t0 k1)
+              | @VisF _ _ _ X e ke => Vis e (fun x : X => ITree.bind (ke x) k1)
+              end).
+    { apply bisimulation_is_eq; rewrite unfold_bind; reflexivity. }
+    rewrite H; clear H.
+
+    assert (ITree.bind t2 k2 =
+              match observe t2 with
+              | RetF r => k2 r
+              | TauF t0 => Tau (ITree.bind t0 k2)
+              | @VisF _ _ _ X e ke => Vis e (fun x : X => ITree.bind (ke x) k2)
+              end).
+    { apply bisimulation_is_eq; rewrite unfold_bind; reflexivity. }
+    rewrite H; clear H.
+
+    pstep.
+    induction EQT; eauto; pclearbot.
+    - specialize (EQK _ _ REL).
+      punfold EQK.
+      eapply interp_PropTF_mono. 1 : eapply EQK. all : eauto.
+      intros. pclearbot. left.
+      eapply paco2_mon; eauto.
+      intros; contradiction.
+    - constructor. right.
+      specialize (CIH _ _ _ _ HS EQK).
+      eauto.
+    - econstructor; auto.
+    - econstructor; auto.
+    - eapply Interp_PropT_Vis_OOM with (e := e).
+      punfold HT1; red in HT1. remember (observe (vis e k0)).
+      hinduction HT1 before U; intros; inv Heqi; try inv CHECK.
+      dependent destruction H1. unfold subevent.
+      eapply eqit_Vis.
+      Unshelve.
+      2 : exact (fun a => bind (k0 a) k1).
+      intros. cbn.
+      eapply eq_itree_clo_bind; pclearbot; eauto. intros; subst; reflexivity.
+    - eapply Interp_PropT_Vis; eauto.
+      intros; eauto. right. eapply CIH; eauto.
+      specialize (HK _ H1). pclearbot. eapply HK; eauto.
+      rewrite <- unfold_bind.
+      setoid_rewrite <- Eq.bind_bind.
+      eapply eutt_clo_bind; eauto. intros; eauto. subst; reflexivity.
+  Qed.
+
+  Lemma interp_prop_mono:
+    forall (R : Type) RR RR' t1 t2,
+      (RR <2= RR') ->
+      interp_prop h RR t1 t2 ->
+      interp_prop h (F := F) (R1 := R1) (R2 := R2) RR' t1 t2.
+  Proof.
+    intros ? ? ?.
+    pcofix self. pstep. intros u v ? euv. punfold euv.
+    red in euv |- *. induction euv; pclearbot; eauto 7 with paco.
+    econstructor; eauto.
+    intros. specialize (HK _ H2). pclearbot.
+    right. eapply self; eauto.
+  Qed.
 
   (* Figure 7: Interpreter law for Ret *)
   Lemma interp_prop_ret :
     forall R (r : R),
-      (interp_prop eq h_spec k_spec (ret r) ≈ ret r)%monad.
+      (interp_prop (F := F) h eq (ret r) ≈ ret r)%monad.
   Proof.
     intros.
     repeat red.
@@ -610,6 +579,7 @@ Section interp_prop_extra.
         * eapply IHinterp_PropTF; eauto.
           assert (Tau t2 ≈ y) by (pstep; auto). rewrite tau_eutt in H1.
           punfold H1; auto.
+        * rewrite itree_eta in HT1; rewrite H1 in HT1; apply eqit_inv in HT1; contradiction.
       + do 2 red in H0. rewrite <- H in H0. clear H.
         punfold H0; red in H0; cbn in H0.
         pstep; red; cbn.
@@ -621,41 +591,42 @@ Section interp_prop_extra.
     - do 3 red. intros. split; intros; cbn in *. rewrite <- H. assumption. rewrite H; assumption.
   Qed.
 
-  From ITree Require Import Eq.EqAxiom.
-
   Lemma interp_prop_bind_refine:
-      forall (R : Type) (t : itree E R) (k : R -> itree E R) (y : itree F R),
-        (x0 <- interp_prop eq h_spec k_spec t;; interp_prop eq h_spec k_spec (k x0)) y -> interp_prop eq h_spec k_spec (x <- t;; k x) y.
+      forall (t : itree E R1) (k : R1 -> itree E R2) (y : itree F R2),
+        (x0 <- interp_prop h eq t;; interp_prop h eq (k x0)) y ->
+        interp_prop h eq (x <- t;; k x) y.
   Proof.
-    intros R t k y H0.
+    intros t k y H0.
     destruct H0 as (x0&x1&?&?&?).
-    rewrite H0. clear H0. clear y.
+    rewrite H0. clear H0 y.
+    rename x0 into t', x1 into k'.
     setoid_rewrite unfold_bind.
     match goal with
-    | |- interp_prop _ _ _ ?l ?r => remember l; remember r
+    | |- interp_prop _ _ ?l ?r => remember l; remember r
     end.
-    revert_until R. pcofix CIH. intros.
+    revert_until RR. pcofix CIH. intros.
     red in H0.
     punfold H0; red in H0; cbn in H0.
-    (* clear x. *)
-    rename t into x, x2 into x'.
-    rename x3 into k', i0 into i'.
-    remember (observe x); remember (observe x').
-    revert_until H0. revert x x' Heqi1 Heqi2.
+    remember (observe t); remember (observe t').
+    setoid_rewrite (itree_eta t') in H1.
+    revert t t' k k' Heqi1 Heqi2 H1 i i0 Heqi Heqi0.
     induction H0; intros.
-    - subst; eauto. setoid_rewrite (itree_eta x') in H1.
-      rewrite <- Heqi2 in H1.
-      assert (Returns (E := F) r2 (Ret r2)) by (econstructor; reflexivity).
+
+    - subst; eauto.
+      assert (Returns r2 t').
+      { rewrite itree_eta; rewrite <- Heqi2; constructor; reflexivity. }
+      setoid_rewrite <- itree_eta in H1.
       specialize (H1 _ H). eapply paco2_mon. punfold H1.
       intros; inv PR.
+
     - (* coinductive tau *)
       pstep. subst. constructor. right. eapply CIH. eauto. pclearbot.
       3,4:eapply bisimulation_is_eq; rewrite unfold_bind; reflexivity.
       pclearbot. punfold HS. pstep. eapply HS.
-      intros; eapply H1. rewrite (itree_eta x').
+      intros; eapply H1. rewrite (itree_eta t').
       rewrite <- Heqi2. eapply ReturnsTau; eauto. reflexivity.
     - rewrite Heqi. pstep. constructor; auto.
-      specialize (IHinterp_PropTF t1 x' eq_refl Heqi2 H1 (bind t1 k)).
+      specialize (IHinterp_PropTF t1 t' k k' eq_refl Heqi2 H1 (bind t1 k)).
 
       assert (H' : x <- t1;; k x =
                   match observe t1 with
@@ -666,14 +637,18 @@ Section interp_prop_extra.
       {
         apply bisimulation_is_eq; setoid_rewrite unfold_bind; reflexivity.
       }
-      specialize (IHinterp_PropTF H' _ Heqi0).
+      specialize (IHinterp_PropTF i0 H' Heqi0).
       punfold IHinterp_PropTF.
     - rewrite Heqi0. pstep. constructor; auto.
-      specialize (IHinterp_PropTF _ t2 Heqi1 eq_refl).
-      assert (forall a : R, Returns a t2 -> interp_prop eq h_spec k_spec (k a) (k' a)).
-      { intros; eapply H1. rewrite (itree_eta x'); rewrite <- Heqi2.
-        rewrite tau_eutt; auto. }
-      specialize (IHinterp_PropTF H _ Heqi (bind t2 k')).
+
+      specialize (IHinterp_PropTF _ _ k k' Heqi1 eq_refl).
+
+      assert (forall a , Returns a t2 -> interp_prop h eq (k a) (k' a)).
+      { intros; eapply H1. rewrite (itree_eta t'); rewrite <- Heqi2.
+        rewrite tau_eutt; auto. rewrite <- itree_eta; auto. }
+
+      setoid_rewrite <- itree_eta in IHinterp_PropTF.
+      specialize (IHinterp_PropTF H).
 
       assert (H' : x <- t2;; k' x =
                   match observe t2 with
@@ -684,38 +659,48 @@ Section interp_prop_extra.
       {
         apply bisimulation_is_eq; setoid_rewrite unfold_bind; reflexivity.
       }
-      specialize (IHinterp_PropTF H').
+      specialize (IHinterp_PropTF _ _ Heqi H').
       punfold IHinterp_PropTF.
-    - rewrite Heqi. pstep. econstructor; [ eauto | ..].
-      + intros.
-        pclearbot.
-        right. eapply CIH; [ auto | ..].
-        3,4 :eapply bisimulation_is_eq; setoid_rewrite <- unfold_bind; reflexivity.
-        eauto. specialize (HK _ H). pclearbot. eapply HK.
-        intros; eapply H1. rewrite (itree_eta x'). rewrite <- Heqi2.
-        eapply k_spec_Returns. 3 : exact H. 3 : exact H0.
-        eauto. eapply k_spec_Proper; eauto. rewrite <- itree_eta; reflexivity.
-      + match goal with
-        | |- k_spec _ _ _ _ ?l _ => remember l
-        end.
-        assert (i0 = (fun a => k2 a >>= k')). {
-          apply FunctionalExtensionality.functional_extensionality.
-          intros; apply bisimulation_is_eq. rewrite Heqi3.
-          rewrite <- unfold_bind; reflexivity.
-        }
-        assert (i' = t2 >>= k'). {
-          apply bisimulation_is_eq. rewrite Heqi0.
-          setoid_rewrite unfold_bind; reflexivity.
-        }
-        eapply k_spec_Proper; eauto.
-        rewrite itree_eta; rewrite H0; rewrite <- itree_eta; reflexivity.
-        rewrite H.
-        eapply k_spec_bind; eauto.
+
+    - subst.
+      punfold HT1.
+      red in HT1. cbn in HT1.
+      remember (VisF (subevent A e) k1).
+      hinduction HT1 before e; intros; inv Heqi.
+      + dependent destruction H2.
+        pclearbot. pstep.
+        eapply Interp_PropT_Vis_OOM; eauto.
+        reflexivity.
+      + pstep. constructor; eauto.
+
+        assert (t0 >>= k =
+                  match observe t0 with
+                  | RetF r => k r
+                  | TauF t0 => Tau (ITree.bind t0 k)
+                  | @VisF _ _ _ X e ke => Vis e (fun x : X => ITree.bind (ke x) k)
+                  end). {
+          intros; apply bisimulation_is_eq.
+          rewrite <- unfold_bind; reflexivity. }
+        setoid_rewrite H.
+
+        specialize (IHHT1 _ eq_refl _ _ _ _ eq_refl H1).
+        punfold IHHT1.
+
+    - rewrite Heqi, Heqi0; clear Heqi Heqi0.
+      pstep. eapply Interp_PropT_Vis; eauto.
+      intros. specialize (HK _ H2); pclearbot. right.
+      eapply CIH; eauto.
+      intros; eapply H1; eauto.
+      rewrite <- Heqi2. rewrite <- itree_eta.
+      rewrite H0. eapply Returns_bind; eauto.
+      apply bisimulation_is_eq; rewrite <- unfold_bind; reflexivity.
+      apply bisimulation_is_eq; setoid_rewrite <- unfold_bind; reflexivity.
+      setoid_rewrite <- unfold_bind. rewrite H0. setoid_rewrite Eq.bind_bind; reflexivity.
   Qed.
 
   Lemma interp_prop_ret_pure :
     forall {T} (RR : relation T) `{REF: Reflexive _ RR} (x : T),
-      interp_prop RR h_spec k_spec (ret x) (ret x).
+      interp_prop (F := F) h RR (ret x) (ret x).
   Proof.
     intros.
     generalize dependent x.
@@ -730,7 +715,7 @@ Section interp_prop_extra.
   Lemma interp_prop_ret_refine :
     forall {T} (RR : relation T) (x y : T),
       RR x y ->
-      interp_prop RR h_spec k_spec (ret x) (ret y).
+      interp_prop (F := F) h RR (ret x) (ret y).
   Proof.
     intros.
     generalize dependent y.
@@ -744,15 +729,15 @@ Section interp_prop_extra.
 
   (* Lemma 5.4: interp_prop_correct - note that the paper presents a slightly simpler formulation where t = t' *)
   Lemma interp_prop_correct_exec:
-    forall (h: E ~> itree F)
-      (HC : handler_correct h_spec h)
-      (KC : k_spec_correct h k_spec),
-      forall R RR `{Reflexive _ RR} (t : _ R) t', t ≈ t' -> interp_prop RR h_spec k_spec t (interp h t').
+    forall {R} RR `{Reflexive _ RR} (t : _ R) t' (f : (forall T : Type, E T -> itree F T))
+      (HC : handler_correct h f),
+      t ≈ t' ->
+      interp_prop h RR t (interp f t').
   Proof.
-    intros h HC KC R RR' H t t' H1.
+    intros R RR0 H t t' f HC H1.
     setoid_rewrite unfold_interp.
-    remember (_interp h (observe t')).
-    assert (i ≅ _interp h (observe t')). {
+    remember (_interp f (observe t')).
+    assert (i ≅ _interp f (observe t')). {
       rewrite Heqi. reflexivity.
     } clear Heqi.
     revert t t' i H1 H0.
@@ -770,14 +755,14 @@ Section interp_prop_extra.
       constructor; auto.
       right; eauto. eapply CIH; pclearbot; eauto.
       rewrite <- unfold_interp; auto.
-    - econstructor.
-      apply HC; reflexivity.
-      intros; right; eapply CIH; eauto.
-      Unshelve.
-      3 : exact (fun x => _interp h (observe (k2 x))).
-      reflexivity.
-      eapply KC; [ reflexivity | rewrite H2].
-      eapply eutt_clo_bind; [ reflexivity | intros; subst; rewrite tau_eutt, unfold_interp; reflexivity].
+    - cbn in H2.
+      eapply Interp_PropT_Vis; eauto; cycle 1.
+      apply HC; reflexivity. rewrite H2.
+      eapply eutt_clo_bind; try reflexivity.
+      intros; subst; setoid_rewrite tau_eutt at 1.
+      Unshelve. 3 : exact (fun x => interp f (k2 x)). reflexivity.
+      intros. right; eapply CIH; eauto.
+      rewrite <- unfold_interp; reflexivity.
     - constructor; auto; eapply IHeq; eauto.
     - cbn in H2.
       apply eqitree_inv_Tau_r in H2.
@@ -788,125 +773,100 @@ Section interp_prop_extra.
 
   (* Figure 7: interp Trigger law *)
   (* morally, we should only work with "proper" triggers everywhere *)
-  Lemma interp_prop_trigger :
-    forall R (e : E R) (HProper: Proper (eutt eq ==> iff) (h_spec _ e)) h
-      (HC : handler_correct h_spec h)
-      (KC : k_spec_correct h k_spec),
-      (interp_prop eq h_spec k_spec (trigger e) ≈ h_spec _ e)%monad.
-  Proof.
-    intros; red.
-    split; [| split]; cycle 1.
-    { do 3 red. intros; split; intros; [rewrite <- H | rewrite H] ; auto. }
-    { do 3 red. intros. split; intros; cbn in *.
-      rewrite <- H. assumption. rewrite H; assumption. }
+  (* Lemma interp_prop_trigger : *)
+  (*   forall R (e : E R) (h : E ~> PropT (itree F)) (HProper: forall A e, Proper (eutt eq ==> iff) (h A e)), *)
+  (*     (interp_prop h eq (trigger e) ≈ h _ e)%monad. *)
+  (* Proof. *)
+  (*   intros; red. *)
+  (*   split; [| split]; cycle 1. *)
+  (*   { do 3 red. intros; split; intros; [rewrite <- H | rewrite H] ; auto. } *)
+  (*   { do 3 red. intros. split; intros; cbn in *. *)
+  (*     rewrite <- H. assumption. rewrite H; assumption. } *)
 
-    intros; split; intros;
-      [rewrite <- H | rewrite <- H in H0]; clear H y.
-    - unfold trigger in H0. red in H0.
-      punfold H0. red in H0. cbn in H0.
-      unfold subevent, resum, ReSum_id, Id_IFun, id_ in H0.
-      remember (VisF e (fun x => Ret x)).
-      rewrite itree_eta.
-      remember (observe x).
-      revert Heqi x Heqi0.
-      induction H0; intros; inv Heqi.
-      + rewrite tau_eutt; rewrite (itree_eta). eapply IHinterp_PropTF; eauto.
-      + dependent destruction H1.
-        assert (x <- ta ;; k2 x ≈ ta).
-        { rewrite <- (Eq.bind_ret_r ta).
-          apply eutt_clo_bind with (UU := fun u1 u2 => u1 = u2 /\ Returns u1 ta).
-          rewrite Eq.bind_ret_r. apply eutt_Returns.
-          intros. destruct H; eauto. subst. specialize (HK _ H0).
-          pclearbot.
-          punfold HK; red in HK; cbn in HK.
-          symmetry.
-          pstep. red. cbn.
-          remember (RetF u2); remember (observe (k2 u2)).
-          assert (go i0 ≈ k2 u2).
-          { rewrite Heqi1, <- itree_eta; reflexivity. }
-          clear Heqi0. clear x H. clear k2 KS Heqi1.
-          revert u2 Heqi H0.
-          revert ta HTA t2.
-          induction HK; intros; inv Heqi.
-          - constructor; auto.
-          - constructor; eauto. }
-        rewrite <- H in HTA. red in HC, KC. symmetry in H.
-        rewrite <- H in HTA.
-        eapply k_spec_respects_h_spec; eauto.
-        eapply k_spec_Proper; eauto. rewrite <- itree_eta; reflexivity.
-      - unfold trigger, subevent, resum, ReSum_id, Id_IFun, id_.
-        red. pstep. eapply Interp_PropT_Vis with (k2 := (fun x : R => Ret x)); eauto.
-        + intros; left; pstep; constructor; auto.
-        + red in KC. eapply KC. eapply HC in H0. eauto.
-          rewrite bind_ret_r; reflexivity.
+  (*   intros; split; intros; *)
+  (*     [rewrite <- H | rewrite <- H in H0]; clear H y. *)
+  (*   - unfold trigger in H0. red in H0. *)
+  (*     punfold H0. red in H0. cbn in H0. *)
+  (*     unfold subevent, resum, ReSum_id, Id_IFun, id_ in H0. *)
+  (*     remember (VisF e (fun x => Ret x)). *)
+  (*     rewrite itree_eta. *)
+  (*     remember (observe x). *)
+  (*     revert Heqi x Heqi0. *)
+      (* induction H0; intros; inv Heqi. *)
+      (* + rewrite tau_eutt; rewrite (itree_eta). eapply IHinterp_PropTF; eauto. *)
+      (* + dependent destruction H1. *)
+      (*   assert (x <- ta ;; k2 x ≈ ta). *)
+      (*   { rewrite <- (Eq.bind_ret_r ta). *)
+      (*     apply eutt_clo_bind with (UU := fun u1 u2 => u1 = u2 /\ Returns u1 ta). *)
+      (*     rewrite Eq.bind_ret_r. apply eutt_Returns. *)
+      (*     intros. destruct H; eauto. subst. specialize (HK _ H0). *)
+      (*     pclearbot. *)
+      (*     punfold HK; red in HK; cbn in HK. *)
+      (*     symmetry. *)
+      (*     pstep. red. cbn. *)
+      (*     remember (RetF u2); remember (observe (k2 u2)). *)
+      (*     assert (go i0 ≈ k2 u2). *)
+      (*     { rewrite Heqi1, <- itree_eta; reflexivity. } *)
+      (*     clear Heqi0. clear x H. clear k2 KS Heqi1. *)
+      (*     revert u2 Heqi H0. *)
+      (*     revert ta HTA t2. *)
+      (*     induction HK; intros; inv Heqi. *)
+      (*     - constructor; auto. *)
+      (*     - constructor; eauto. } *)
+      (*   rewrite <- H in HTA. red in HC, KC. symmetry in H. *)
+      (*   rewrite <- H in HTA. *)
+      (*   eapply k_spec_WF_respects_h_spec; eauto. *)
+      (*   eapply k_spec_WF_Proper; eauto. rewrite <- itree_eta; reflexivity. *)
+      (* - unfold trigger, subevent, resum, ReSum_id, Id_IFun, id_. *)
+      (*   red. pstep. eapply Interp_PropT_Vis with (k2 := (fun x : R => Ret x)); eauto. *)
+      (*   + intros; left; pstep; constructor; auto. *)
+      (*   + red in KC. eapply KC. eapply HC in H0. eauto. *)
+      (*     rewrite bind_ret_r; reflexivity. *)
+  (* Admitted. *)
+
+  Lemma interp_prop_ret_inv:
+    forall  r1 (t : itree F _),
+      interp_prop (F := F) h RR (ret r1) t -> exists r2 , RR r1 r2 /\ t ≈ ret r2.
+  Proof.
+    intros r1 t INTERP.
+    punfold INTERP.
+    red in INTERP.
+    setoid_rewrite itree_eta with (t:=t).
+    remember (observe (ret r1)); remember (observe t).
+    clear Heqi0.
+    induction INTERP; subst; pclearbot; intros.
+    - exists r2.
+      cbn in Heqi.
+      inv Heqi.
+      split; auto.
+      cbn.
+      reflexivity.
+    - inv Heqi.
+    - inv Heqi.
+    - cbn in INTERP.
+      inv INTERP.
+      + apply simpobs in H.
+        exists r2; split; auto.
+        rewrite H.
+        rewrite tau_eutt.
+        reflexivity.
+      + specialize (IHINTERP eq_refl).
+        destruct IHINTERP as [r2 [RRr1r2 EQ]].
+        exists r2; split; auto.
+        rewrite <- itree_eta in EQ.
+        rewrite EQ.
+        rewrite tau_eutt.
+        reflexivity.
+      + setoid_rewrite tau_eutt.
+        specialize (IHINTERP eq_refl).
+        destruct IHINTERP as [r2 [RRr1r2 EQ]].
+        exists r2; split; auto.
+        rewrite <- itree_eta in EQ.
+        rewrite EQ.
+        reflexivity.
+    - inv Heqi.
+      rewrite itree_eta in HT1; rewrite H0 in HT1; apply eqit_inv in HT1; contradiction.
+    - inv Heqi.
   Qed.
 
 End interp_prop_extra.
-
-Lemma interp_prop_ret_inv:
-  forall (E F : Type -> Type) (h_spec : forall T : Type, E T -> PropT F T)
-    (k_spec : forall T R : Type,
-        E T -> itree F T -> (T -> itree F R) -> itree F R -> Prop) 
-    (R : Type) (RR : Relation_Definitions.relation R) (r1 : R) (t : itree F R),
-    interp_prop RR h_spec k_spec (ret r1) t -> exists r2 : R, RR r1 r2 /\ t ≈ ret r2.
-Proof.
-  intros E F h_spec k_spec R RR r1 t INTERP.
-  punfold INTERP.
-  red in INTERP.
-  setoid_rewrite itree_eta with (t:=t).
-  remember (observe (ret r1)); remember (observe t).
-  clear Heqi0.
-  induction INTERP; subst; pclearbot; intros.
-  - exists r2.
-    cbn in Heqi.
-    inv Heqi.
-    split; auto.
-    cbn.
-    reflexivity.
-  - inv Heqi.
-  - inv Heqi.
-  - cbn in INTERP.
-    inv INTERP.
-    + apply simpobs in H.
-      exists r2; split; auto.
-      rewrite H.
-      rewrite tau_eutt.
-      reflexivity.
-    + specialize (IHINTERP eq_refl).
-      destruct IHINTERP as [r2 [RRr1r2 EQ]].
-      exists r2; split; auto.
-      rewrite <- itree_eta in EQ.
-      rewrite EQ.
-      rewrite tau_eutt.
-      reflexivity.
-  - inv Heqi.
-Qed.
-
-Section interp_refl.
-
-  Lemma interp_prop_refl_h :
-    forall {T E} (RR : relation T) `{REF: Reflexive _ RR} (t1 t2 : itree E T)
-      (h : E ~> PropT E)
-      (k_spec : forall T R, E T -> itree E T -> (T -> itree E R) -> itree E R -> Prop),
-      (forall {X : Type} (e : E X), h X e (trigger e)) ->
-      (k_spec_correct (fun T e => trigger e) k_spec) ->
-      t1 ≈ t2 ->
-      interp_prop RR h k_spec t1 t2.
-  Proof.
-  Admitted.
-
-  Lemma interp_prop_refl :
-    forall {T E} (RR : relation T) `{REF: Reflexive _ RR} (t : itree E T)
-      (h : forall X : Type, E X -> PropT E X)
-      (k_spec : forall T R, E T -> itree E T -> (T -> itree E R) -> itree E R -> Prop),
-      (forall {X : Type} (e : E X), h X e (trigger e)) ->
-      (k_spec_correct (fun T e => trigger e) k_spec) ->
-      interp_prop RR h k_spec t t.
-  Proof.
-    intros T E0 RR REF t h k_spec H_SPEC K_SPEC.
-    apply interp_prop_refl_h; eauto.
-    reflexivity.
-  Qed.
-
-End interp_refl.
-
