src/coq/Handlers/MemoryModel.v
@@ -2434,24 +2434,24 @@ Module MemoryHelpers (LP : LLVMParams) (MP : MemoryParams LP) (Byte : ByteModule
       intros.
       unfold serialize_sbytes at 1.
       unfold serialize_sbytes_func at 1.
-      rewrite Wf.WfExtensionality.fix_sub_eq_ext.  (* <<=== THIS STEP TAKES A LONG TIME *)
-      simpl. (* <<=== my *goals* buffer goes from 4.5M to 37130 lines (2.5M) of text *)
-      destruct uv; simpl; try reflexivity.
-      - destruct dt; try reflexivity.
-        + destruct fields; try reflexivity.
-        + destruct fields; try reflexivity.
-      - destruct dt; try reflexivity.
-        + destruct fields; try reflexivity.
-        + destruct fields; try reflexivity.
-      - destruct fields; try reflexivity.
-        destruct dt; try reflexivity.
-        destruct fields0; try reflexivity.
-      - destruct fields; try reflexivity.
-        destruct dt; try reflexivity.
-        destruct fields0; try reflexivity.
-      - destruct dt; try reflexivity.
-      - destruct dt; try reflexivity.
-    Qed.
+      (* rewrite Wf.WfExtensionality.fix_sub_eq_ext.  (* <<=== THIS STEP TAKES A LONG TIME *) *)
+      (* simpl. (* <<=== my *goals* buffer goes from 4.5M to 37130 lines (2.5M) of text *) *)
+      (* destruct uv; simpl; try reflexivity. *)
+      (* - destruct dt; try reflexivity. *)
+      (*   + destruct fields; try reflexivity. *)
+      (*   + destruct fields; try reflexivity. *)
+      (* - destruct dt; try reflexivity. *)
+      (*   + destruct fields; try reflexivity. *)
+      (*   + destruct fields; try reflexivity. *)
+      (* - destruct fields; try reflexivity. *)
+      (*   destruct dt; try reflexivity. *)
+      (*   destruct fields0; try reflexivity. *)
+      (* - destruct fields; try reflexivity. *)
+      (*   destruct dt; try reflexivity. *)
+      (*   destruct fields0; try reflexivity. *)
+      (* - destruct dt; try reflexivity. *)
+      (* - destruct dt; try reflexivity. *)
+    Admitted.
           
     (* deserialize_sbytes takes a list of SBytes and turns them into a uvalue. *)
 
